PREFIX : <https://def.isotc211.org/common/CouplingType/>
PREFIX cs: <https://def.isotc211.org/common/CouplingType>
PREFIX schema: <https://schema.org/>
PREFIX skos: <http://www.w3.org/2004/02/skos/core#>
PREFIX status: <https://def.isotc211.org/RE/ItemStatus/>
PREFIX xsd: <http://www.w3.org/2001/XMLSchema#>

:loose
    a skos:Concept ;
    skos:definition "service instance is loosely coupled with a data instance, i.e. no DataIdentification class has to be described"@en ;
    skos:historyNote "Originally presented in the ISO 19115-1:2014 standard codelist, reproduced unchanged here"@en ;
    skos:inScheme cs: ;
    skos:prefLabel "loose"@en ;
    skos:topConceptOf cs: ;
    schema:status status:original ;
    rdfs:isDefinedBy <https://def.isotc211.org/SV/CouplingType> ;
.

:mixed
    a skos:Concept ;
    skos:definition "service instance is mixed coupled with a data instance, i.e. DataIdentification describes the associated data instance and additionally the service instance might work with other external data instances"@en ;
    skos:historyNote "Originally presented in the ISO 19115-1:2014 standard codelist, reproduced unchanged here"@en ;
    skos:inScheme cs: ;
    skos:prefLabel "mixed"@en ;
    skos:topConceptOf cs: ;
    schema:status status:original ;
    rdfs:isDefinedBy <https://def.isotc211.org/SV/CouplingType> ;
.

:tight
    a skos:Concept ;
    skos:definition "service instance is tightly coupled with a data instance, i.e. DataIdentification class MUST be described"@en ;
    skos:historyNote "Originally presented in the ISO 19115-1:2014 standard codelist, reproduced unchanged here"@en ;
    skos:inScheme cs: ;
    skos:prefLabel "tight"@en ;
    skos:topConceptOf cs: ;
    schema:status status:original ;
    rdfs:isDefinedBy <https://def.isotc211.org/SV/CouplingType> ;
.

cs:
    a skos:ConceptScheme ;
    skos:definition "class of information to which the referencing entity applies"@en ;
    skos:hasTopConcept
        :loose ,
        :mixed ,
        :tight ;
    skos:historyNote "This version of this codeset was produced for the 2025 update of the 19115 standard" ;
    skos:prefLabel "Coupling Type"@en ;
    schema:creator <https://def.isotc211.org/org/tc211> ;
    schema:dateCreated "2025-11-19"^^xsd:date ;
    schema:dateIssued "2025-11-19"^^xsd:date ;
    schema:dateModified "2025-11-19"^^xsd:date ;
    schema:isPartOf <https://def.isotc211.org/common> ;
    schema:publisher <https://def.isotc211.org/org/tc211> ;
    schema:status status:experimental ;
    rdfs:isDefinedBy <https://def.isotc211.org/common/standard/iso-awi-19115-1> ;
.
