PREFIX : <https://def.isotc211.org/common/KeywordTypeCode/>
PREFIX cs: <https://def.isotc211.org/common/KeywordTypeCode>
PREFIX prov: <http://www.w3.org/ns/prov#>
PREFIX schema: <https://schema.org/>
PREFIX skos: <http://www.w3.org/2004/02/skos/core#>
PREFIX status: <https://def.isotc211.org/RE/ItemStatus/>
PREFIX xsd: <http://www.w3.org/2001/XMLSchema#>

:dataCentre
    a skos:Concept ;
    skos:definition "keyword identifies a a repository or archive that manages and distributes data"@en ;
    skos:historyNote "Originally presented in the XXXX standard codelist, reproduced unchanged here"@en ;
    skos:inScheme cs: ;
    skos:prefLabel "data centre"@en ;
    skos:topConceptOf cs: ;
    schema:status status:original ;
.

:discipline
    a skos:Concept ;
    skos:definition "keyword identifies a branch of instruction or specialized learning"@en ;
    skos:historyNote "Originally presented in the XXXX standard codelist, reproduced unchanged here"@en ;
    skos:inScheme cs: ;
    skos:prefLabel "discipline"@en ;
    skos:topConceptOf cs: ;
    schema:status status:original ;
.

:featureType
    a skos:Concept ;
    skos:definition "keyword identifies a resource containing or about a collection of feature instances with common characteristics"@en ;
    skos:historyNote "Originally presented in the XXXX standard codelist, reproduced unchanged here"@en ;
    skos:inScheme cs: ;
    skos:prefLabel "feature type"@en ;
    skos:topConceptOf cs: ;
    schema:status status:original ;
.

:instrument
    a skos:Concept ;
    skos:definition "keyword identifies a device used to measure or compare physical properties"@en ;
    skos:historyNote "Originally presented in the XXXX standard codelist, reproduced unchanged here"@en ;
    skos:inScheme cs: ;
    skos:prefLabel "instrument"@en ;
    skos:topConceptOf cs: ;
    schema:status status:original ;
.

:place
    a skos:Concept ;
    skos:definition "keyword identifies a location"@en ;
    skos:historyNote "Originally presented in the XXXX standard codelist, reproduced unchanged here"@en ;
    skos:inScheme cs: ;
    skos:prefLabel "place"@en ;
    skos:topConceptOf cs: ;
    schema:status status:original ;
.

:platform
    a skos:Concept ;
    skos:definition "keyword identifies a structure upon which an instrument is mounted"@en ;
    skos:historyNote "Originally presented in the XXXX standard codelist, reproduced unchanged here"@en ;
    skos:inScheme cs: ;
    skos:prefLabel "platform"@en ;
    skos:topConceptOf cs: ;
    schema:status status:original ;
.

:process
    a skos:Concept ;
    skos:definition "keyword identifies a series of actions or natural occurrences"@en ;
    skos:historyNote "Originally presented in the XXXX standard codelist, reproduced unchanged here"@en ;
    skos:inScheme cs: ;
    skos:prefLabel "process"@en ;
    skos:topConceptOf cs: ;
    schema:status status:original ;
.

:product
    a skos:Concept ;
    skos:definition "keyword identifies a type of product"@en ;
    skos:historyNote "Originally presented in the XXXX standard codelist, reproduced unchanged here"@en ;
    skos:inScheme cs: ;
    skos:prefLabel "product"@en ;
    skos:topConceptOf cs: ;
    schema:status status:original ;
.

:project
    a skos:Concept ;
    skos:definition "keyword identifies an endeavour undertaken to create or modify a product or service"@en ;
    skos:historyNote "Originally presented in the XXXX standard codelist, reproduced unchanged here"@en ;
    skos:inScheme cs: ;
    skos:prefLabel "project"@en ;
    skos:topConceptOf cs: ;
    schema:status status:original ;
.

:service
    a skos:Concept ;
    skos:definition "keyword identifies an activity carried out by one party for the benefit of another"@en ;
    skos:historyNote "Originally presented in the XXXX standard codelist, reproduced unchanged here"@en ;
    skos:inScheme cs: ;
    skos:prefLabel "service"@en ;
    skos:topConceptOf cs: ;
    schema:status status:original ;
.

:stratum
    a skos:Concept ;
    skos:definition "keyword identifies the layer(s) of any deposited substance or levels within an ordered system"@en ;
    skos:historyNote "Originally presented in the XXXX standard codelist, reproduced unchanged here"@en ;
    skos:inScheme cs: ;
    skos:prefLabel "stratum"@en ;
    skos:topConceptOf cs: ;
    schema:status status:original ;
.

:subTopicCategory
    a skos:Concept ;
    skos:definition "refinement of a topic category for the purpose of geographic data classification"@en ;
    skos:historyNote "Originally presented in the XXXX standard codelist, reproduced unchanged here"@en ;
    skos:inScheme cs: ;
    skos:prefLabel "sub topic category"@en ;
    skos:topConceptOf cs: ;
    schema:status status:original ;
.

:taxon
    a skos:Concept ;
    skos:definition "keyword identifies a taxonomy of the resource"@en ;
    skos:historyNote "Originally presented in the XXXX standard codelist, reproduced unchanged here"@en ;
    skos:inScheme cs: ;
    skos:prefLabel "taxon"@en ;
    skos:topConceptOf cs: ;
    schema:status status:original ;
.

:temporal
    a skos:Concept ;
    skos:definition "keyword identifies a time period related to the resource"@en ;
    skos:historyNote "Originally presented in the XXXX standard codelist, reproduced unchanged here"@en ;
    skos:inScheme cs: ;
    skos:prefLabel "temporal"@en ;
    skos:topConceptOf cs: ;
    schema:status status:original ;
.

:theme
    a skos:Concept ;
    skos:definition "keyword identifies a particular subject or topic"@en ;
    skos:historyNote "Originally presented in the XXXX standard codelist, reproduced unchanged here"@en ;
    skos:inScheme cs: ;
    skos:prefLabel "theme"@en ;
    skos:topConceptOf cs: ;
    schema:status status:original ;
.

cs:
    a skos:ConceptScheme ;
    skos:definition "methods used to group similar keywords"@en ;
    skos:hasTopConcept
        :dataCentre ,
        :discipline ,
        :featureType ,
        :instrument ,
        :place ,
        :platform ,
        :process ,
        :product ,
        :project ,
        :service ,
        :stratum ,
        :subTopicCategory ,
        :taxon ,
        :temporal ,
        :theme ;
    skos:historyNote "This version of this codeset was produced for the 2025 update of the 19115 standard" ;
    skos:prefLabel "Keyword Type Code"@en ;
    schema:creator <https://def.isotc211.org/org/tc211> ;
    schema:dateCreated "2025-11-19"^^xsd:date ;
    schema:dateIssued "2025-11-19"^^xsd:date ;
    schema:dateModified "2025-11-19"^^xsd:date ;
    schema:isPartOf <https://def.isotc211.org/common> ;
    schema:publisher <https://def.isotc211.org/org/tc211> ;
    schema:status status:experimental ;
    prov:wasDerivedFrom <https://def.isotc211.org/common/standard/iso-awi-19115-1> ;
.
