PREFIX : <https://def.isotc211.org/common/ReferenceSystemTypeCode/>
PREFIX cs: <https://def.isotc211.org/common/ReferenceSystemTypeCode>
PREFIX schema: <https://schema.org/>
PREFIX skos: <http://www.w3.org/2004/02/skos/core#>
PREFIX status: <https://def.isotc211.org/RE/ItemStatus/>
PREFIX xsd: <http://www.w3.org/2001/XMLSchema#>

:compoundEngineeringParametric
    a skos:Concept ;
    skos:definition "compound statio-parametric coordinate reference system containing an engineering coordinate reference system and a parametric reference system e.g. [local] x, y, pressure"@en ;
    skos:historyNote "Originally presented in the ISO 19115-1:2014 standard codelist, reproduced unchanged here"@en ;
    skos:inScheme cs: ;
    skos:prefLabel "compound engineering parametric"@en ;
    skos:topConceptOf cs: ;
    schema:status status:original ;
    rdfs:isDefinedBy <https://def.isotc211.org/MD/ReferenceSystemTypeCode> ;
.

:compoundEngineeringParametricTemporal
    a skos:Concept ;
    skos:definition "compound statio-parametric-temporal coordinate reference system containing an engineering, a parametric, and a temporal coordinate reference system e.g. [local] x, y, pressure, time"@en ;
    skos:historyNote "Originally presented in the ISO 19115-1:2014 standard codelist, reproduced unchanged here"@en ;
    skos:inScheme cs: ;
    skos:prefLabel "compound engineering parametric temporal"@en ;
    skos:topConceptOf cs: ;
    schema:status status:original ;
    rdfs:isDefinedBy <https://def.isotc211.org/MD/ReferenceSystemTypeCode> ;
.

:compoundEngineeringTemporal
    a skos:Concept ;
    skos:definition "compound spatio-temoral coordinate reference system containing an engineering and a temporal coordinate reference system e.g. [local] x, y, time"@en ;
    skos:historyNote "Originally presented in the ISO 19115-1:2014 standard codelist, reproduced unchanged here"@en ;
    skos:inScheme cs: ;
    skos:prefLabel "compound engineering temporal"@en ;
    skos:topConceptOf cs: ;
    schema:status status:original ;
    rdfs:isDefinedBy <https://def.isotc211.org/MD/ReferenceSystemTypeCode> ;
.

:compoundEngineeringVertical
    a skos:Concept ;
    skos:definition "compound spatial reference system containing a horizontal engineering coordinate reference system and a vertical coordinate reference system e.g. [local] x, y, height"@en ;
    skos:historyNote "Originally presented in the ISO 19115-1:2014 standard codelist, reproduced unchanged here"@en ;
    skos:inScheme cs: ;
    skos:prefLabel "compound engineering vertical"@en ;
    skos:topConceptOf cs: ;
    schema:status status:original ;
    rdfs:isDefinedBy <https://def.isotc211.org/MD/ReferenceSystemTypeCode> ;
.

:compoundEngineeringVerticalTemporal
    a skos:Concept ;
    skos:definition "compound spatio-temoral coordinate reference system containing an engineering, a vertical, and a temporal coordinate reference system e.g. [local] x, y, height, time"@en ;
    skos:historyNote "Originally presented in the ISO 19115-1:2014 standard codelist, reproduced unchanged here"@en ;
    skos:inScheme cs: ;
    skos:prefLabel "compound engineering vertical temporal"@en ;
    skos:topConceptOf cs: ;
    schema:status status:original ;
    rdfs:isDefinedBy <https://def.isotc211.org/MD/ReferenceSystemTypeCode> ;
.

:compoundGeographic2DParametric
    a skos:Concept ;
    skos:definition "compound statio-parametric coordinate reference system containing a 2 dimensional geographic horizontal coordinate reference system and a parametric reference system e.g. latitude, longitude, pressure"@en ;
    skos:historyNote "Originally presented in the ISO 19115-1:2014 standard codelist, reproduced unchanged here"@en ;
    skos:inScheme cs: ;
    skos:prefLabel "compound geographic2 d parametric"@en ;
    skos:topConceptOf cs: ;
    schema:status status:original ;
    rdfs:isDefinedBy <https://def.isotc211.org/MD/ReferenceSystemTypeCode> ;
.

:compoundGeographic2DParametricTemporal
    a skos:Concept ;
    skos:definition "compound statio-parametric-temporal coordinate reference system containing a 2 dimensional geographic horizontal, a parametric and a temporal coordinate reference system e.g. latitude, longitude, pressure, time"@en ;
    skos:historyNote "Originally presented in the ISO 19115-1:2014 standard codelist, reproduced unchanged here"@en ;
    skos:inScheme cs: ;
    skos:prefLabel "compound geographic2 d parametric temporal"@en ;
    skos:topConceptOf cs: ;
    schema:status status:original ;
    rdfs:isDefinedBy <https://def.isotc211.org/MD/ReferenceSystemTypeCode> ;
.

:compoundGeographic2DTemporal
    a skos:Concept ;
    skos:definition "compound spatio-temoral coordinate reference system containing a 2 dimensional geographic horizontal coordinate reference system and a temporal reference system e.g. latitude, longitude, time"@en ;
    skos:historyNote "Originally presented in the ISO 19115-1:2014 standard codelist, reproduced unchanged here"@en ;
    skos:inScheme cs: ;
    skos:prefLabel "compound geographic2 d temporal"@en ;
    skos:topConceptOf cs: ;
    schema:status status:original ;
    rdfs:isDefinedBy <https://def.isotc211.org/MD/ReferenceSystemTypeCode> ;
.

:compoundGeographic2DVertical
    a skos:Concept ;
    skos:definition "compound coordinate reference system in which one constituent coordinate reference system is a horizontal geodetic coordinate reference system and one is a vertical coordinate reference system e.g. latitude, longitude, [gravity-related] height or depth"@en ;
    skos:historyNote "Originally presented in the ISO 19115-1:2014 standard codelist, reproduced unchanged here"@en ;
    skos:inScheme cs: ;
    skos:prefLabel "compound geographic2 d vertical"@en ;
    skos:topConceptOf cs: ;
    schema:status status:original ;
    rdfs:isDefinedBy <https://def.isotc211.org/MD/ReferenceSystemTypeCode> ;
.

:compoundGeographic2DVerticalTemporal
    a skos:Concept ;
    skos:definition "compound spatio-temoral coordinate reference system containing a 2 dimensional geographic horizontal, a vertical, and a temporal coordinate reference system e.g. latitude, longitude, height, time"@en ;
    skos:historyNote "Originally presented in the ISO 19115-1:2014 standard codelist, reproduced unchanged here"@en ;
    skos:inScheme cs: ;
    skos:prefLabel "compound geographic2 d vertical temporal"@en ;
    skos:topConceptOf cs: ;
    schema:status status:original ;
    rdfs:isDefinedBy <https://def.isotc211.org/MD/ReferenceSystemTypeCode> ;
.

:compoundGeographic3DTemporal
    a skos:Concept ;
    skos:definition "compound spatio-temoral coordinate reference system containing a 3 dimensional geographic and a temporal coordinate reference system e.g. latitude, longitude, ellipsoidal height, time"@en ;
    skos:historyNote "Originally presented in the ISO 19115-1:2014 standard codelist, reproduced unchanged here"@en ;
    skos:inScheme cs: ;
    skos:prefLabel "compound geographic3 d temporal"@en ;
    skos:topConceptOf cs: ;
    schema:status status:original ;
    rdfs:isDefinedBy <https://def.isotc211.org/MD/ReferenceSystemTypeCode> ;
.

:compoundProjected2DParametric
    a skos:Concept ;
    skos:definition "compound statio-parametric coordinate reference system containing a projected horizontal coordinate reference system and a parametric reference system e.g. easting, northing, density"@en ;
    skos:historyNote "Originally presented in the ISO 19115-1:2014 standard codelist, reproduced unchanged here"@en ;
    skos:inScheme cs: ;
    skos:prefLabel "compound projected2 d parametric"@en ;
    skos:topConceptOf cs: ;
    schema:status status:original ;
    rdfs:isDefinedBy <https://def.isotc211.org/MD/ReferenceSystemTypeCode> ;
.

:compoundProjected2DParametricTemporal
    a skos:Concept ;
    skos:definition "compound statio-parametric-temporal coordinate reference system containing a projected horizontal, a parametric, and a temporal coordinate reference system e.g. easting, northing, density, time"@en ;
    skos:historyNote "Originally presented in the ISO 19115-1:2014 standard codelist, reproduced unchanged here"@en ;
    skos:inScheme cs: ;
    skos:prefLabel "compound projected2 d parametric temporal"@en ;
    skos:topConceptOf cs: ;
    schema:status status:original ;
    rdfs:isDefinedBy <https://def.isotc211.org/MD/ReferenceSystemTypeCode> ;
.

:compoundProjectedTemporal
    a skos:Concept ;
    skos:definition "compound spatio-temoral coordinate reference system containing a projected horizontal and a temporal coordinate reference system e.g. easting, northing, time"@en ;
    skos:historyNote "Originally presented in the ISO 19115-1:2014 standard codelist, reproduced unchanged here"@en ;
    skos:inScheme cs: ;
    skos:prefLabel "compound projected temporal"@en ;
    skos:topConceptOf cs: ;
    schema:status status:original ;
    rdfs:isDefinedBy <https://def.isotc211.org/MD/ReferenceSystemTypeCode> ;
.

:compoundProjectedVertical
    a skos:Concept ;
    skos:definition "compound spatial reference system containing a horizontal projected coordinate reference system and a vertical coordinate reference system e.g. easting, northing, [gravity-related] height or depth"@en ;
    skos:historyNote "Originally presented in the ISO 19115-1:2014 standard codelist, reproduced unchanged here"@en ;
    skos:inScheme cs: ;
    skos:prefLabel "compound projected vertical"@en ;
    skos:topConceptOf cs: ;
    schema:status status:original ;
    rdfs:isDefinedBy <https://def.isotc211.org/MD/ReferenceSystemTypeCode> ;
.

:compoundProjectedVerticalTemporal
    a skos:Concept ;
    skos:definition "compound spatio-temoral coordinate reference system containing a projected horizontal, a vertical, and a temporal coordinate reference system e.g. easting, northing, height, time"@en ;
    skos:historyNote "Originally presented in the ISO 19115-1:2014 standard codelist, reproduced unchanged here"@en ;
    skos:inScheme cs: ;
    skos:prefLabel "compound projected vertical temporal"@en ;
    skos:topConceptOf cs: ;
    schema:status status:original ;
    rdfs:isDefinedBy <https://def.isotc211.org/MD/ReferenceSystemTypeCode> ;
.

:engineering
    a skos:Concept ;
    skos:definition "coordinate reference system based on an engineering datum (datum describing the relationship of a coordinate system to a local reference)e.g. [local] x,y"@en ;
    skos:historyNote "Originally presented in the ISO 19115-1:2014 standard codelist, reproduced unchanged here"@en ;
    skos:inScheme cs: ;
    skos:prefLabel "engineering"@en ;
    skos:topConceptOf cs: ;
    schema:status status:original ;
    rdfs:isDefinedBy <https://def.isotc211.org/MD/ReferenceSystemTypeCode> ;
.

:engineeringDesign
    a skos:Concept ;
    skos:definition "engineering coordinate reference system in which the base representation of a moving object is specified e.g. [local] x,y"@en ;
    skos:historyNote "Originally presented in the ISO 19115-1:2014 standard codelist, reproduced unchanged here"@en ;
    skos:inScheme cs: ;
    skos:prefLabel "engineering design"@en ;
    skos:topConceptOf cs: ;
    schema:status status:original ;
    rdfs:isDefinedBy <https://def.isotc211.org/MD/ReferenceSystemTypeCode> ;
.

:engineeringImage
    a skos:Concept ;
    skos:definition "coordinate reference system based on an image datum (engineering datum which defines the relationship of a coordinate system to an image)e.g. row, column"@en ;
    skos:historyNote "Originally presented in the ISO 19115-1:2014 standard codelist, reproduced unchanged here"@en ;
    skos:inScheme cs: ;
    skos:prefLabel "engineering image"@en ;
    skos:topConceptOf cs: ;
    schema:status status:original ;
    rdfs:isDefinedBy <https://def.isotc211.org/MD/ReferenceSystemTypeCode> ;
.

:geodeticGeocentric
    a skos:Concept ;
    skos:definition "geodetic CRS having a Cartesian 3D coordinate system e.g. [geocentric] X,Y,Z"@en ;
    skos:historyNote "Originally presented in the ISO 19115-1:2014 standard codelist, reproduced unchanged here"@en ;
    skos:inScheme cs: ;
    skos:prefLabel "geodetic geocentric"@en ;
    skos:topConceptOf cs: ;
    schema:status status:original ;
    rdfs:isDefinedBy <https://def.isotc211.org/MD/ReferenceSystemTypeCode> ;
.

:geodeticGeographic2D
    a skos:Concept ;
    skos:definition "geodetic CRS having an ellipsoidal 2D coordinate system e.g. latitude, longitude"@en ;
    skos:historyNote "Originally presented in the ISO 19115-1:2014 standard codelist, reproduced unchanged here"@en ;
    skos:inScheme cs: ;
    skos:prefLabel "geodetic geographic2 d"@en ;
    skos:topConceptOf cs: ;
    schema:status status:original ;
    rdfs:isDefinedBy <https://def.isotc211.org/MD/ReferenceSystemTypeCode> ;
.

:geodeticGeographic3D
    a skos:Concept ;
    skos:definition "geodetic CRS having an ellipsoidal 3D coordinate system e.g. latitude, longitude, ellipsoidal height"@en ;
    skos:historyNote "Originally presented in the ISO 19115-1:2014 standard codelist, reproduced unchanged here"@en ;
    skos:inScheme cs: ;
    skos:prefLabel "geodetic geographic3 d"@en ;
    skos:topConceptOf cs: ;
    schema:status status:original ;
    rdfs:isDefinedBy <https://def.isotc211.org/MD/ReferenceSystemTypeCode> ;
.

:geographicIdentifier
    a skos:Concept ;
    skos:definition "spatial reference in the form of a label or code that identifies a location e.g. post code"@en ;
    skos:historyNote "Originally presented in the ISO 19115-1:2014 standard codelist, reproduced unchanged here"@en ;
    skos:inScheme cs: ;
    skos:prefLabel "geographic identifier"@en ;
    skos:topConceptOf cs: ;
    schema:status status:original ;
    rdfs:isDefinedBy <https://def.isotc211.org/MD/ReferenceSystemTypeCode> ;
.

:linear
    a skos:Concept ;
    skos:definition "reference system that identifies a location by reference to a segment of a linear geographic feature and distance along that segment from a given point e.g. x km along road"@en ;
    skos:historyNote "Originally presented in the ISO 19115-1:2014 standard codelist, reproduced unchanged here"@en ;
    skos:inScheme cs: ;
    skos:prefLabel "linear"@en ;
    skos:topConceptOf cs: ;
    schema:status status:original ;
    rdfs:isDefinedBy <https://def.isotc211.org/MD/ReferenceSystemTypeCode> ;
.

:parametric
    a skos:Concept ;
    skos:definition "coordinate reference system based on a parametric datum (datum describing the relationship of a parametric coordinate system to an object) e.g. pressure"@en ;
    skos:historyNote "Originally presented in the ISO 19115-1:2014 standard codelist, reproduced unchanged here"@en ;
    skos:inScheme cs: ;
    skos:prefLabel "parametric"@en ;
    skos:topConceptOf cs: ;
    schema:status status:original ;
    rdfs:isDefinedBy <https://def.isotc211.org/MD/ReferenceSystemTypeCode> ;
.

:projected
    a skos:Concept ;
    skos:definition "coordinate reference system derived from a two-dimensional geodetic coordinate reference system by applying a map projection e.g. easting, northing"@en ;
    skos:historyNote "Originally presented in the ISO 19115-1:2014 standard codelist, reproduced unchanged here"@en ;
    skos:inScheme cs: ;
    skos:prefLabel "projected"@en ;
    skos:topConceptOf cs: ;
    schema:status status:original ;
    rdfs:isDefinedBy <https://def.isotc211.org/MD/ReferenceSystemTypeCode> ;
.

:temporal
    a skos:Concept ;
    skos:definition "reference system against which time is measured e.g. time"@en ;
    skos:historyNote "Originally presented in the ISO 19115-1:2014 standard codelist, reproduced unchanged here"@en ;
    skos:inScheme cs: ;
    skos:prefLabel "temporal"@en ;
    skos:topConceptOf cs: ;
    schema:status status:original ;
    rdfs:isDefinedBy <https://def.isotc211.org/MD/ReferenceSystemTypeCode> ;
.

:vertical
    a skos:Concept ;
    skos:definition "one-dimensional coordinate reference system based on a vertical datum (datum describing the relation of gravity-related heights or depths to the Earth) e.g. [gravity-related] height or depth"@en ;
    skos:historyNote "Originally presented in the ISO 19115-1:2014 standard codelist, reproduced unchanged here"@en ;
    skos:inScheme cs: ;
    skos:prefLabel "vertical"@en ;
    skos:topConceptOf cs: ;
    schema:status status:original ;
    rdfs:isDefinedBy <https://def.isotc211.org/MD/ReferenceSystemTypeCode> ;
.

cs:
    a skos:ConceptScheme ;
    skos:definition "defines type of reference system used"@en ;
    skos:hasTopConcept
        :compoundEngineeringParametric ,
        :compoundEngineeringParametricTemporal ,
        :compoundEngineeringTemporal ,
        :compoundEngineeringVertical ,
        :compoundEngineeringVerticalTemporal ,
        :compoundGeographic2DParametric ,
        :compoundGeographic2DParametricTemporal ,
        :compoundGeographic2DTemporal ,
        :compoundGeographic2DVertical ,
        :compoundGeographic2DVerticalTemporal ,
        :compoundGeographic3DTemporal ,
        :compoundProjected2DParametric ,
        :compoundProjected2DParametricTemporal ,
        :compoundProjectedTemporal ,
        :compoundProjectedVertical ,
        :compoundProjectedVerticalTemporal ,
        :engineering ,
        :engineeringDesign ,
        :engineeringImage ,
        :geodeticGeocentric ,
        :geodeticGeographic2D ,
        :geodeticGeographic3D ,
        :geographicIdentifier ,
        :linear ,
        :parametric ,
        :projected ,
        :temporal ,
        :vertical ;
    skos:historyNote "This version of this codeset was produced for the 2025 update of the 19115 standard" ;
    skos:prefLabel "Reference System Type Code"@en ;
    schema:creator <https://def.isotc211.org/org/tc211> ;
    schema:dateCreated "2025-11-19"^^xsd:date ;
    schema:dateIssued "2025-11-19"^^xsd:date ;
    schema:dateModified "2025-11-19"^^xsd:date ;
    schema:isPartOf <https://def.isotc211.org/common> ;
    schema:publisher <https://def.isotc211.org/org/tc211> ;
    schema:status status:experimental ;
    rdfs:isDefinedBy <https://def.isotc211.org/common/standard/iso-awi-19115-1> ;
.
